Changed naming in ordseq

refinements/ordseq.v
@@ -1,64 +1,87 @@
 (** This file is part of CoqEAL, the Coq Effective Algebra Library.
 (c) Copyright INRIA and University of Gothenburg, see LICENSE *)
 
-Require Import ZArith.
-
 From mathcomp Require Import all_ssreflect.
 
 From CoqEAL Require Import hrel param refinements.
 
 Import Refinements.Op.
 
+Section Classes.
+
+(* cardinality, union, intersection, complement, asymmetric difference *)
+Class card_of fset :=
+  card_op : forall n : nat, fset n -> nat.
+Class union_of fset :=
+  union_op : forall n : nat, fset n -> fset n -> fset n.
+Class inter_of fset :=
+  inter_op : forall n : nat, fset n -> fset n -> fset n.
+Class compl_of fset :=
+  compl_op : forall n : nat, fset n -> fset n.
+Class adiff_of fset :=
+  adiff_op : forall n : nat, fset n -> fset n -> fset n.
+(* Null set, singleton, subset *)
+Class empty_of fset :=
+  empty_op : forall n : nat, fset n.
+Class singl_of fset :=
+  singl_op : forall n : nat, nat -> fset n.
+Class subset_of fset :=
+  subset_op : forall n : nat, fset n -> fset n -> bool.
+
+End Classes.
+
 (** ordseq.v: An implementation of sets of ordinals as sorted sequences
     of nats containing unique elements *)
-Local Open Scope computable_scope.
 
 Section ordseq_op.
 
-(* Variable A : eqType. *)
+(* Number Type *)
 Variable N : Type.
 
-Definition ordseq := fun (_ : nat) => seq nat.
+(* Set type *)
+Variable F : nat -> Type.
 
 Context `{zero_of N, one_of N, add_of N, eq_of N, leq_of N, lt_of N, spec_of N nat}.
+Context `{implem_of nat N}.
 
-Global Instance ordseq0 {m} : zero_of (ordseq m) := [::].
-Global Instance eq_ordseq {m} : eq_of (ordseq m) := @eqseq nat_eqType.
+Definition ordseq := @seq nat.
+Definition hset := fun (_ : nat) => ordseq.
 
-Fixpoint ordseq_sublist {m} (p q : ordseq m) : bool :=
-  (* mem_aux : returns true/false, plus the remaining list after the match
-               in case the element has indeed been found *)
-  let fix mem_aux x (p' : ordseq m) : bool * (ordseq m) := match p' with
-  | [::] => (false, [::])
-  | h :: t =>
-      (* If element is found, return true and the rest of the other set *)
-      if (h == x) then (true, t)
-      else mem_aux x t
-  end
-  in
-  match p with
-  | [::] => true
-  | h :: t => match mem_aux h q with
-    | (false, _) => false
-    | (true, t') => ordseq_sublist t t'
-    end
+(* Inlining of && should provide lazyness here. *)
+Fixpoint eq_seq {T} f (s1 s2 : seq T) :=
+  match s1, s2 with
+  | [::], [::] => true
+  | x1 :: s1', x2 :: s2' => f x1 x2 && eq_seq f s1' s2'
+  | _, _ => false
   end.
 
-Definition ordseq_sub {m} : sub_of (ordseq m) :=
-  let fix aux a b := match b with
-  | [::] => a
-  | h :: t => aux (rem h a) t
-  end in aux.
+Global Instance ordseq0 : empty_of hset := fun _ => [::].
+Global Instance ordseq_eq : eq_of ordseq := @eqseq nat_eqType.
 
-Lemma ordseq_sub_nil {m} (I : ordseq m) :
-  ordseq_sub I [::] = I.
+Global Instance ordseq_card : card_of hset :=
+  fun _ M => seq.size M.
+
+Global Instance ordseq_singleton : singl_of hset :=
+  fun _ e => [:: e].
+
+Global Instance ordseq_adiff : adiff_of hset :=
+  fix aux _ p q := match q with
+  | [::] => p
+  | h :: t => aux _ (rem h p) t
+  end.
+
+Global Instance ordseq_union : union_of hset :=
+  fun _ a b => merge leq a (ordseq_adiff _ b a).
+
+Lemma ordseq_adiff_nil {m} (I : hset m) :
+  ordseq_adiff _ I [::] = I.
 Proof. by elim: I. Qed.
 
-Lemma ordseq_nil_sub {m} (I : ordseq m) :
-  ordseq_sub [::] I = [::].
+Lemma ordseq_nil_adiff {m} (I : hset m) :
+  ordseq_adiff _ [::] I = [::].
 Proof. by elim: I. Qed.
 
-Lemma rem_sorted {m} (I : ordseq m) (i : nat) :
+Lemma rem_sorted {m} (I : hset m) (i : nat) :
   sorted leq I -> sorted leq (rem i I).
 Proof.
   move: (rem_subseq i I) => Hsub HsI.
@@ -68,113 +91,98 @@ Proof.
     exact: HsI ].
 Qed.
 
-Lemma ordseq_sub_sorted {m} (I J : ordseq m) :
-  sorted leq I -> sorted leq J -> sorted leq (ordseq_sub I J).
+Lemma ordseq_adiff_sorted {m} (I J : hset m) :
+  sorted leq I -> sorted leq J -> sorted leq (ordseq_adiff _ I J).
 Proof.
   elim: J I => [// | j J Hind] [// | i I] //.
-  - move => _ _. by rewrite ordseq_nil_sub.
-  - move => HsI HsJ. rewrite /ordseq_sub.
+  - move => _ _. by rewrite ordseq_nil_adiff.
+  - move => HsI HsJ. rewrite /ordseq_adiff.
     have Hs: sorted leq (rem j (i :: I)) by apply: (@rem_sorted m).
     apply: Hind; first by exact: Hs.
     move: (subseq_cons J j) => Hcons. apply: subseq_sorted;
     [ exact: leq_trans | exact: Hcons | exact: HsJ].
 Qed.
 
-Lemma ordseq_sub_uniq {m} (I J : ordseq m) :
-  uniq I -> uniq J -> uniq (ordseq_sub I J).
+Lemma ordseq_adiff_uniq {m} (I J : hset m) :
+  uniq I -> uniq J -> uniq (ordseq_adiff _ I J).
 Proof.
   elim: J I => [// | j J Hind] [// | i I] //.
-  - move => _ _; by rewrite ordseq_nil_sub.
+  - move => _ _; by rewrite ordseq_nil_adiff.
   - move => HuI. rewrite cons_uniq; move => /andP[_ HuJ].
     have Hu: uniq (rem j (i :: I)) by apply: rem_uniq.
-    apply: Hind; first by exact: Hu.
-    done.
+    apply: Hind; [ exact: Hu | done ].
 Qed.
 
-Lemma rem_is_sub {m} (I : ordseq m) :
+Lemma rem_is_sub {m} (I : hset m) :
   forall i, i \in I -> i \notin rem i I.
 Proof.
   move => i. elim: I => [// | hi I Hind].
 Admitted.
 
-Lemma ordseq_sub_is_sub {m} (I J : ordseq m) (i : nat) :
-  i \in ordseq_sub I J -> i \in I /\ i \notin J.
+Lemma ordseq_adiff_is_adiff {m} (I J : hset m) (i : nat) :
+  i \in ordseq_adiff _ I J -> i \in I /\ i \notin J.
 Proof.
   elim: J I => [// | j J Hind] [// | hi I] //.
-  - by rewrite ordseq_nil_sub //=.
+  - by rewrite ordseq_nil_adiff //=.
   - admit.
   (* This is too much *)
 Admitted.
 
-
-(* Union of two ordseqs *)
-Definition ordseq_add {m} : add_of (ordseq m) :=
-  fun a b => merge leq a (ordseq_sub b a).
-
-Lemma ordseq_add_sorted {m} (I J : ordseq m) :
-  sorted leq I -> sorted leq J -> sorted leq (ordseq_add I J).
+Lemma ordseq_union_sorted {m} (I J : hset m) :
+  sorted leq I -> sorted leq J -> sorted leq (ordseq_union _ I J).
 Proof.
   move => Hi Hj. apply: merge_sorted.
   - rewrite /total => x y. case/boolP: (x <= y)%N => //.
     by rewrite -ltnNge ltn_neqAle => /andP[_ ?].
   - exact: Hi.
-  - exact: ordseq_sub_sorted.
+  - exact: ordseq_adiff_sorted.
 Qed.
 
-Lemma ordseq_add_nil {m} (I : ordseq m) :
-  ordseq_add I [::] = I.
+Lemma ordseq_union_nil {m} (I : hset m) :
+  ordseq_union _ I [::] = I.
 Proof.
-  rewrite /ordseq_add ordseq_nil_sub; by elim: I.
+  rewrite /ordseq_union ordseq_nil_adiff; by elim: I.
 Qed.
 
-Lemma ordseq_nil_add {m} (I : ordseq m) :
-  ordseq_add [::] I = I.
+Lemma ordseq_nil_union {m} (I : hset m) :
+  ordseq_union _ [::] I = I.
 Proof.
-  rewrite /ordseq_add; by elim: I.
+  rewrite /ordseq_union; by elim: I.
 Qed.
 
-Lemma ordseq_add_is_union {m} (I J : ordseq m) :
+Lemma ordseq_union_is_union {m} (I J : hset m) :
   sorted leq I -> sorted leq J ->
-  forall (i : nat), (i \in ordseq_add I J) -> i \in I \/ i \in J.
+  forall (i : nat), (i \in ordseq_union _ I J) -> i \in I \/ i \in J.
 Proof.
   move => Hi Hj i; case Icomp: I.
-  - rewrite ordseq_nil_add => ?; by apply/orP.
-  - rewrite /ordseq_add mem_merge mem_cat.
+  - rewrite ordseq_nil_union => ?; by apply/orP.
+  - rewrite /ordseq_union mem_merge mem_cat.
     move/orP; case => Hin; apply/orP.
     - by rewrite Hin.
     - move: Hin; rewrite -Icomp => Hsub.
-      have : i \in J /\ (i \notin I) by exact: ordseq_sub_is_sub.
+      have : i \in J /\ (i \notin I) by exact: ordseq_adiff_is_adiff.
       move => [Hj' _]; by rewrite Hj' orbT.
 Qed.
 
 (** Returning if an element is a member of a set *)
-Fixpoint ordseq_mem {m} x (p : ordseq m) : bool := match p with
+Fixpoint ordseq_mem {m} x (p : hset m) : bool := match p with
   | [::] => false
   | h :: t => (h == x) || @ordseq_mem m x t
   end.
 
-Global Instance implem_ordseq {m} : implem_of {set 'I_m} (ordseq m) :=
+Global Instance implem_ordseq {m} : implem_of {set 'I_m} (hset m) :=
   fun s => [seq (nat_of_ord i) | i <- enum s].
 
-(* TODO: We need a spec_of nat 'I_m somehow! *)
 Global Instance spec_ordseq {m} `{H : spec_of nat 'I_m} :
-  spec_of (@ordseq m) {set 'I_m} := fun s =>
+  spec_of (@hset m) {set 'I_m} := fun s =>
   let sMapped := map (@spec _ _ H) s in
   [set i | i \in sMapped].
-
-(** Size of a set *)
-Global Instance size_seqset {m} : size_of (ordseq m) N :=
-  let fix aux cnt p := match p with
-  | [::] => cnt
-  | _ :: t => aux (cnt + 1) t
-  end
-  in aux 0.
 
 Local Open Scope rel_scope.
 
 (* In the spirit of Rseqmx...*)
 CoInductive Rordseq {m1 m2} (rm : nat_R m1 m2) :
-  {set 'I_m1} -> @ordseq m2 -> Type := Rordseq_spec (I : {set 'I_m1}) (J : ordseq m2) of
+  {set 'I_m1} -> @hset m2 -> Type := Rordseq_spec (I : {set 'I_m1}) (J : hset m2) of
   (forall j, j \in J -> (j < m1)%N) &
   (uniq J) & (sorted leq J) : Rordseq rm I J.
 
@@ -191,46 +199,45 @@ Lemma in_ordseq_sorted {m1 m2} (rm : nat_R m1 m2) I J :
 Proof. by case. Qed.
 
 Instance Rordseq_sub {m1 m2} (rm : nat_R m1 m2)
-(I : 'I_m1) (J : (@ordseq m2)) :
+(I : 'I_m1) (J : (@hset m2)) :
   refines (Rordseq rm ==> Rordseq rm ==> Rordseq rm)
-  (@setD (ordinal_finType m1)) (@ordseq_sub m2).
+  (@setD (ordinal_finType m1)) (@ordseq_adiff m2).
 Proof.
   rewrite refinesE => I' J' Ho Ialt Jalt Ho' //=; constructor.
   - move => j Hj.
-    have : (j \in J') /\ j \notin Jalt. apply: ordseq_sub_is_sub.
+    have : (j \in J') /\ j \notin Jalt. apply: ordseq_adiff_is_adiff.
     + exact: Hj.
     move => [Hj' _].
     have -> : forall j, j \in J' -> (j < m1)%N. case: Ho => _.
     + move => J0 Hex _ _ j0 Hjex. exact: Hex.
     + rewrite //=.
     + exact: Hj'.
-  - apply: ordseq_sub_uniq; [
+  - apply: ordseq_adiff_uniq; [
       exact: in_ordseq_uniq Ho |
       exact: in_ordseq_uniq Ho' ]. 
-  - apply: ordseq_sub_sorted; [
+  - apply: ordseq_adiff_sorted; [
       exact: (in_ordseq_sorted rm I' J') |
       exact: (in_ordseq_sorted rm Ialt Jalt) ].
 Qed.
 
 Instance Rordseq_add {m1 m2} (rm : nat_R m1 m2)
-(I : 'I_m1) (J : (@ordseq m2)) :
+(I : 'I_m1) (J : (@hset m2)) :
   refines (Rordseq rm ==> Rordseq rm ==> Rordseq rm)
-  (@setU (ordinal_finType m1)) (@ordseq_add m2).
+  (@setU (ordinal_finType m1)) (@ordseq_union m2).
 Proof.
   rewrite refinesE => I' J' Ho Ialt Jalt Ho'; constructor.
   - move => j Hjadd. have : j \in J' \/ j \in Jalt.
-    + apply: ordseq_add_is_union.
+    + apply: ordseq_union_is_union.
       * apply: (in_ordseq_sorted _ _ J'); exact: Ho.
       * apply: (in_ordseq_sorted _ _ Jalt); exact: Ho'.
       * exact: Hjadd.
     + case; apply: in_ordseq_lt; [exact: Ho | exact: Ho'].
-  - rewrite /ordseq_add merge_uniq cat_uniq; apply/and3P; split.
+  - rewrite merge_uniq cat_uniq; apply/and3P; split.
     + exact: (in_ordseq_uniq rm I' J').
-    + apply/hasPn => x Hnot. have [_ ->] : x \in Jalt /\ x \notin J'.
-      * by exact: ordseq_sub_is_sub.
-      * done.
-    + apply: ordseq_sub_uniq; [
+    + apply/hasPn => x Hnot. have [_ ->] : x \in Jalt /\ x \notin J';
+      [ exact: ordseq_adiff_is_adiff | done ].
+    + apply: ordseq_adiff_uniq; [
       exact: in_ordseq_uniq Ho' | exact: in_ordseq_uniq Ho ].
-  - apply: ordseq_add_sorted; apply: in_ordseq_sorted;
+  - apply: ordseq_union_sorted; apply: in_ordseq_sorted;
     [ exact: Ho | exact: Ho' ].
 Qed.
